No need for depth now

Source/DafnyRuntime/dafnySequence.dfy
@@ -13,39 +13,30 @@ module {:options "/functionSyntax:4"} MetaSeq {
     | Empty
     | Direct(a: seq<T>)
     | Concat(left: SeqExpr<T>, right: SeqExpr<T>, length: nat)
-    | Lazy(ghost value: seq<T>, ghost boxDepth: nat, ghost boxSize: nat,
+    | Lazy(ghost value: seq<T>, ghost boxSize: nat,
            exprBox: AtomicBox<SeqExpr<T>>, length: nat) 
   {
     ghost predicate Valid()
-      decreases Depth(), 0
+      decreases Size(), 0
     {
       match this
       case Concat(left, right, length) => 
         && left.Valid()
         && right.Valid()
         && left.Length() + right.Length() == length
-      case Lazy(value, depth, size, exprBox, length) => 
+      case Lazy(value, size, exprBox, length) => 
         && length == |value|
         && exprBox.inv == ((e: SeqExpr<T>) => 
-          && e.Depth() < depth 
           && e.Size() < size
           && e.Valid() 
           && e.Value() == value)
       case _ => true
     }
 
-    ghost function Depth(): nat {
-      match this {
-        case Concat(left, right, _) => 1 + Math.Max(left.Depth(), right.Depth())
-        case Lazy(_, depth, _, _, _) => depth
-        case _ => 0
-      }
-    }
-
     ghost function Size(): nat {
       match this {
         case Concat(left, right, _) => 1 + left.Size() + right.Size()
-        case Lazy(_, _, boxSize, _, _) => 1 + boxSize
+        case Lazy(_, boxSize, _, _) => 1 + boxSize
         case _ => 1
       }
     }
@@ -55,7 +46,7 @@ module {:options "/functionSyntax:4"} MetaSeq {
       case Empty => 0
       case Direct(a) => |a|
       case Concat(_, _, length) => length
-      case Lazy(_, _, _, _, length) => length
+      case Lazy(_, _, _, length) => length
     }
 
     function At(i: nat): T 
@@ -71,14 +62,14 @@ module {:options "/functionSyntax:4"} MetaSeq {
 
     function Value(): seq<T> 
       requires Valid()
-      decreases Depth(), 2
+      decreases Size(), 2
       ensures |Value()| == Length()
     {
       match this
       case Empty => []
       case Direct(a) => a
       case Concat(left, right, length) => left.Value() + right.Value()
-      case Lazy(value, _, _, _, _) => value
+      case Lazy(value, _, _, _) => value
     } by method {
       match this
       case Empty => return [];
@@ -89,7 +80,7 @@ module {:options "/functionSyntax:4"} MetaSeq {
         AppendValue(builder, toAppendAfter);
         return builder.Value();
       }
-      case Lazy(_, _, _, seqExpr, _) => {
+      case Lazy(_, _, seqExpr, _) => {
         var expr := exprBox.Get();
         var value := expr.Value();
         exprBox.Put(Direct(value));
@@ -134,7 +125,7 @@ module {:options "/functionSyntax:4"} MetaSeq {
           assert SizeSum(toAppendAfter.Repr) == old(SizeSum(toAppendAfter.Repr)) + right.Size();
           left.AppendValue(builder, toAppendAfter);
         }
-        case Lazy(_, _, _, exprBox, _) => {
+        case Lazy(_, _, exprBox, _) => {
           var expr := exprBox.Get();
           expr.AppendValue(builder, toAppendAfter);
         }
@@ -153,7 +144,6 @@ module {:options "/functionSyntax:4"} MetaSeq {
     requires (forall e <- s :: e.Valid())
     requires x.Valid()
     ensures ConcatValueOnStack(s + [x]) == x.Value() + ConcatValueOnStack(s)
-    ensures SizeSum(s + [x]) == x.Size() + SizeSum(s)
   {
     var valueFn := (e: SeqExpr<T>) requires e.Valid() => e.Value();
     calc {
